@prefix iot: <http://iot.schema.org/core#> .
@prefix owl: <http://www.w3.org/2002/07/owl#> .
@prefix rdf: <http://www.w3.org/1999/02/22-rdf-syntax-ns#> .
@prefix rdfs: <http://www.w3.org/2000/01/rdf-schema#> .
@prefix schema: <http://schema.org/> .
@prefix xml: <http://www.w3.org/XML/1998/namespace> .
@prefix xsd: <http://www.w3.org/2001/XMLSchema#> .

iot:Action
  rdf:type rdfs:Class ;
  rdfs:comment "Action subclass of InteractionPattern" ;
  rdfs:label "Action" ;
  rdfs:subClassOf iot:InteractionPattern ;
.
iot:Actuator
  rdf:type rdfs:Class ;
  rdfs:comment "Actuator - A device that is used to change the state of the world. " ;
  rdfs:label "Actuator" ;
  rdfs:subClassOf iot:Device ;
.
iot:Capability
  rdf:type rdfs:Class ;
  rdfs:comment "Capability Class" ;
  rdfs:label "Capability" ;
  rdfs:subClassOf schema:Thing ;
.
iot:Domain
  rdf:type rdfs:Class ;
  rdfs:comment "Specifies a domain e.g., Building domain, Mobility domain, or domain agnostic (Common domain)."^^xsd:string ;
  rdfs:label "Domain"^^xsd:string ;
  rdfs:subClassOf schema:Enumeration ;
.
iot:Event
  rdf:type rdfs:Class ;
  rdfs:comment "Event subclass of InteractionPattern" ;
  rdfs:label "Event" ;
  rdfs:subClassOf iot:InteractionPattern ;
.
iot:FeatureOfInterest
  rdf:type rdfs:Class ;
  rdfs:comment "Feature Of Interest - The thing whose property is being estimated or calculated in the course of an Observation, or whose property is being manipulated by an Actuator. " ;
  rdfs:label "FeatureOfInterest" ;
.
iot:InteractionPattern
  rdf:type rdfs:Class ;
  rdfs:comment "General Interaction Pattern Class" ;
  rdfs:label "Interaction Pattern" ;
.
iot:Property
  rdf:type rdfs:Class ;
  rdfs:comment "Property subclass of InteractionPattern" ;
  rdfs:label "Property" ;
  rdfs:subClassOf iot:InteractionPattern ;
.
iot:Sensor
  rdf:type rdfs:Class ;
  rdfs:comment "Sensor - Device, agent (including humans), or software (simulation). Sensors respond to a Stimulus, e.g., a change in the environment, data composed from the Results of prior Observations, and generate a Result." ;
  rdfs:label "Sensor" ;
  rdfs:subClassOf iot:Device ;
.
iot:acceptsInputData
  rdf:type rdf:Property ;
  schema:domainIncludes iot:InteractionPattern ;
  schema:rangeIncludes schema:PropertyValue ;
  schema:rangeIncludes schema:PropertyValueSpecification ;
  rdfs:label "accepts input data" ;
.
iot:domain
  rdf:type rdf:Property ;
  schema:rangeIncludes iot:Domain ;
  rdfs:comment "Specifies a domain e.g., Building domain, Mobility domain, or domain agnostic (Common domain)."^^xsd:string ;
  rdfs:label "domain"^^xsd:string ;
.
iot:providesInterctionPattern
  rdf:type rdf:Property ;
  schema:domainIncludes iot:Capability ;
  schema:rangeIncludes iot:InteractionPattern ;
  rdfs:label "Property for InteractionPattern" ;
.
iot:providesOutputData
  rdf:type rdf:Property ;
  schema:domainIncludes iot:InteractionPattern ;
  schema:rangeIncludes schema:PropertyValue ;
  schema:rangeIncludes schema:PropertyValueSpecification ;
  rdfs:label "Property for Output Data from an Interaction" ;
.
schema:Building
  rdf:type iot:Domain ;
  rdfs:comment "Building Domain"^^xsd:string ;
  rdfs:label "Building"^^xsd:string ;
.
schema:Common
  rdf:type iot:Domain ;
  rdfs:comment "Horizontal Domain (Cross Domain)"^^xsd:string ;
  rdfs:label "Common"^^xsd:string ;
.
schema:Mobility
  rdf:type iot:Domain ;
  rdfs:comment "Mobility Domain"^^xsd:string ;
  rdfs:label "Mobility"^^xsd:string ;
.
iot:Device
  rdf:type rdfs:Class ;
  rdfs:comment "Device Class" ;
  rdfs:label "Device" ;
  rdfs:subClassOf schema:Thing ;
.
iot:resultTime
  rdf:type rdf:Property ;
  schema:domainIncludes iot:PropertyValue ;
  schema:rangeIncludes schema:DateTime ;
  rdfs:label "Result Time" ;
  rdfs:comment "The result time is the instant of time when the Observation or Actuation activity was completed. "^^xsd:string ;
.
iot:phenomenonTime
  rdf:type rdf:Property ;
  schema:domainIncludes iot:PropertyValue ;
  schema:rangeIncludes schema:Duration ;
  schema:rangeIncludes schema:DateTime ;
  rdfs:label "Phenomenon Time" ;
  rdfs:comment "The time that the Result of an Observation or Actuation applies to the FeatureOfInterest. Not necessarily the same as the resultTime. May be an interval or an instant, or some other compound temporal entity [owl-time].  "^^xsd:string ;
.
iot:observes
  rdf:type rdf:Property ;
  schema:domainIncludes iot:Sensor ;
  schema:rangeIncludes iot:Property ;
  schema:rangeIncludes iot:Event ;
  rdfs:label "Observes" ;
  rdfs:comment "Relation between a Sensor and either a Property or an Event that it is capable of sensing."^^xsd:string ;
.
iot:isObservedBy
  rdf:type rdf:Property ;
  schema:domainIncludes iot:Property ;
  schema:domainIncludes iot:Event ;
  schema:rangeIncludes iot:Sensor ;
  rdfs:label "Is Observed By" ;
  rdfs:comment "Relation between a PropertyValue and the Sensor which is able to observe it."^^xsd:string ;
.
iot:forProperty
  rdf:type rdf:Property ;
  schema:domainIncludes iot:Actuator ;
  schema:rangeIncludes iot:Property ;
  schema:rangeIncludes iot:Action ;
  rdfs:label "For Property" ;
  rdfs:comment " Relation between an Actuator and either a Property or an Action that it is capable of actuation. "^^xsd:string ;
.
iot:hasFeatureOfInterest
  rdf:type rdf:Property ;
  schema:domainIncludes schema:PropertyValue ;
  schema:rangeIncludes iot:FeatureOfInterest ;
  rdfs:label "Has Feature Of Interest" ;
  rdfs:comment " A relation between a PropertyValue and the entity whose quality was observed, or whose property was modified."^^xsd:string ;
.
iot:madeObservation
  rdf:type rdf:Property ;
  schema:domainIncludes iot:Sensor ;
  schema:rangeIncludes schema:PropertyValue ;
  rdfs:label "Made Observation" ;
  rdfs:comment " Relation between a Sensor and a PropertyValue it has made. "^^xsd:string ;
.
iot:madeActuation
  rdf:type rdf:Property ;
  schema:domainIncludes iot:Actuator ;
  schema:rangeIncludes schema:PropertyValue ;
  rdfs:label "Made Actuation" ;
  rdfs:comment " Relation linking a PropertyValue to the Actuator that made that Actuation. "^^xsd:string ;
.
iot:observedProperty
  rdf:type rdf:Property ;
  schema:domainIncludes iot:PropertyValue ;
  schema:rangeIncludes schema:Property ;
  schema:rangeIncludes schema:Event ;
  rdfs:label "Observed Property" ;
  rdfs:comment " Relation linking a PropertyValue to the property or Event that was observed. The Property or Event should be a property of the FeatureOfInterest (linked by hasFeatureOfInterest) of this PropertyValue. "^^xsd:string ;
.
iot:actsOnProperty
  rdf:type rdf:Property ;
  schema:domainIncludes iot:PropertyValue ;
  schema:rangeIncludes schema:Property ;
  schema:rangeIncludes schema:Action ;
  rdfs:label "Acts On Property" ;
  rdfs:comment "Relation between a PropertyValue and the Property or Action of a FeatureOfInterest it is acting upon."^^xsd:string ;
.
iot:isActedOnBy
  rdf:type rdf:Property ;
  schema:domainIncludes iot:Property ;
  schema:domainIncludes iot:Action ;  
  schema:rangeIncludes iot:Actuator ;
  rdfs:label "Is Acted On By" ;
  rdfs:comment "Relation between an Action or a Property of a FeatureOfInterest and an Actuator changing its state."^^xsd:string ;
.